coq_ssprove/src/ChoiceEquality.v
@@ -221,6 +221,16 @@ Next Obligation.
   apply r_ret.
   intros ? ? []. easy.
 Defined.
+
+Program Instance prod_both0 {ceA ceB : choice_type} {L : {fset _}} {I : {fset _}} (a : both L I ceA) (b : both L I ceB) : both (L) (I) (ceA × ceB) :=
+  prod_both a b.
+Next Obligation.
+  intros. apply fsetUid.
+Qed.
+Next Obligation.
+  intros. apply fsetUid.
+Qed.
+
 Notation "prod_b( a , b )" := (prod_both a b) : hacspec_scope.
 Notation "prod_b( a , b , .. , c )" := (prod_both .. (prod_both a b) .. c) : hacspec_scope.
 
@@ -784,41 +794,22 @@ Definition prod_to_prod {A B} {L I} (x : both L I (A × B)) : (both L I A * both
                                                     (fun (H H0 : heap) (H1 : true_precond (H, H0)) =>
                                                        conj (conj eq_refl eq_refl) H1))|}).
 
-(* Definition prod_to_prod0 {A B} (x : both0 (A × .. × B)) : (both0 A * both0 B) := prod_to_prod x. *)
+Definition prod_to_prod3 {A B C} {L I} (x : both L I (A × B × C)) : (both L I A * both L I B * both L I C) :=
+  let '(temp, c) := prod_to_prod x in
+  let '(a, b) := prod_to_prod temp in
+  (a, b, c).
 
-Program Definition prod_to_prod_uncurry {A B C} {L I} (f : both L I (A × B) -> both L I C) (x : both L I A) (y : both L I B) : both L I C :=
-  f ({|
-        is_pure := (is_pure x, is_pure y) : choice.Choice.sort (chProd A B) ;
-        is_state :=
-        {code
-           temp_x ← is_state x ;;
-           temp_y ← is_state y ;;
-           ret ((temp_x, temp_y) : choice.Choice.sort (chProd A B))} ;
-      |} : both L I (A × B)).
-Next Obligation.
-  intros.
+Fixpoint split_type (F : choice_type -> Type) (A : choice_type) : Type :=
+  match A with
+  | C × D => split_type F C * split_type F D
+  | _ => F A
+  end.
 
-  replace (ret _) with (temp_x ← ret x ;; temp_y ← ret y ;; ret ((temp_x , temp_y) : choice.Choice.sort (chProd A B))) by reflexivity.
-
-  apply r_bind with (mid := pre_to_post_ret true_precond (is_pure x)).
-  apply (code_eq_proof_statement x).
-  intros.
-
-  apply rpre_hypothesis_rule.
-  intros ? ? [[]] ; subst.
-  apply forget_precond.
-
-  apply r_bind with (mid := pre_to_post_ret true_precond (is_pure y)).
-  apply forget_precond.
-  apply (code_eq_proof_statement y).
-  intros.
-
-  apply rpre_hypothesis_rule.
-  intros ? ? [[]] ; subst.
-  apply forget_precond.
-
-  apply r_ret.
-  intros.
-
-  easy.
-Qed.
+Fixpoint split_both {L I A} (x : both L I A) : split_type (both L I) A :=
+  match A as B return (both L I B -> split_type (both L I) B) with
+  | C × D =>
+      fun y =>
+      let (c,d) := (prod_to_prod y) in
+      (split_both c, split_both d)
+  | _ => fun y => y
+  end x.
